add V1ModelLang and maintain ConcreteHoare proofs

core/ConcreteHoare.v
@@ -4,6 +4,8 @@ Require Import Poulet4.Semantics.
 Require Import ProD3.core.Coqlib.
 Require Import ProD3.core.Hoare.
 Require Import ProD3.core.AssertionLang.
+Require Import Poulet4.V1Model.
+Require Import ProD3.core.V1ModelLang.
 Require Import Hammer.Tactics.Tactics.
 Require Import Hammer.Plugin.Hammer.
 
@@ -19,91 +21,120 @@ Notation path := (list ident).
 Notation P4Int := (P4Int.t tags_t).
 Notation P4String := (P4String.t tags_t).
 Notation signal := (@signal tags_t).
-Notation assertion := (@assertion tags_t).
 Notation arg_assertion := (@arg_assertion tags_t).
 Notation ret_assertion := (@ret_assertion tags_t).
+Notation mem_assertion := (@AssertionLang.assertion tags_t).
+Notation ext_assertion := (@ext_assertion tags_t).
 
-Context `{@Target tags_t (@Expression tags_t)}.
+Notation state := (@state tags_t V1Model).
 
 Variable ge : (@genv tags_t).
 Variable inst_m : (@inst_mem tags_t).
-(* Variable this : path. *)
+
+Section WithThisPath.
+
+Variable this : path.
+
+Definition assertion : Type := mem_assertion * ext_assertion.
 
 Record post_assertion := mk_post_assertion {
   post_continue :> assertion;
-  post_return : ret_assertion * assertion
+  post_return : ret_assertion * mem_assertion * ext_assertion
 }.
 
-Definition to_shallow_post_assertion (p : path) (post : post_assertion) : Hoare.post_assertion :=
-  match post with 
-  | mk_post_assertion a_continue a_return =>
-      Hoare.mk_post_assertion (to_shallow_assertion p a_continue)
-        (fun vret st => ret_to_shallow_assertion (fst a_return) vret /\ to_shallow_assertion p (snd a_return) st)
+Definition to_shallow_assertion_continue (a : assertion) :=
+  match a with (a_mem, a_ext) =>
+  (fun (st : state) => let (m, es) := st in
+    to_shallow_assertion this a_mem m /\
+    ext_to_shallow_assertion this a_ext es)
   end.
 
-Definition hoare_expr (pre : assertion) (expr : Expression) (v : Val) : Prop :=
-  eval_expr ge pre expr = Some v.
+Definition to_shallow_assertion_return (a : ret_assertion * mem_assertion * ext_assertion) :=
+  match a with (a_ret, a_mem, a_ext) =>
+  (fun vret (st : state) => let (m, es) := st in
+    ret_to_shallow_assertion a_ret vret /\
+    to_shallow_assertion this a_mem m /\
+    ext_to_shallow_assertion this a_ext es)
+  end.
 
-Lemma hoare_expr_sound : forall p pre expr v,
-  wellformed pre ->
-  hoare_expr pre expr v ->
-  Hoare.hoare_expr ge p (to_shallow_assertion p pre) expr v.
+Definition to_shallow_post_assertion (post : post_assertion) : Hoare.post_assertion :=
+  match post with mk_post_assertion a_continue a_return =>
+  Hoare.mk_post_assertion (to_shallow_assertion_continue a_continue) (to_shallow_assertion_return a_return)
+  end.
+
+Definition implies (pre : assertion) (post : assertion) : bool :=
+  AssertionLang.implies (fst pre) (fst post) && ext_implies (snd pre) (snd post).
+
+Lemma implies_sound : forall (pre post : assertion),
+  implies pre post ->
+  Hoare.implies (to_shallow_assertion_continue pre) (to_shallow_assertion_continue post).
 Proof.
-  unfold Hoare.hoare_expr; intros.
-  eapply eval_expr_sound; eassumption.
+  intros * H_implies. destruct pre; destruct post.
+  apply Reflect.andE in H_implies. destruct H_implies.
+  intros [] []. split.
+  - eapply AssertionLang.implies_sound; eassumption.
+  - eapply ext_implies_sound; eassumption.
 Qed.
 
-Definition hoare_lexpr (p : path) (pre : assertion) (expr : @Expression tags_t) (lv : Lval) : Prop :=
+Definition hoare_expr (pre : assertion) (expr : Expression) (v : Val) : Prop :=
+  eval_expr ge (fst pre) expr = Some v.
+
+Lemma hoare_expr_sound : forall (pre : assertion) expr v,
+  wellformed (fst pre) ->
+  hoare_expr pre expr v ->
+  Hoare.hoare_expr ge this (to_shallow_assertion_continue pre) expr v.
+Proof.
+  unfold Hoare.hoare_expr; intros.
+  destruct pre; destruct st; destruct H1.
+  eapply eval_expr_sound; try eassumption; eassumption.
+Qed.
+
+Definition hoare_lexpr (pre : assertion) (expr : Expression) (lv : Lval) : Prop :=
   eval_lexpr expr = Some lv.
 
-Lemma hoare_lexpr_sound : forall p pre expr lv,
-  hoare_lexpr p pre expr lv ->
-  Hoare.hoare_lexpr ge p (to_shallow_assertion p pre) expr (lval_to_semlval lv).
+Lemma hoare_lexpr_sound : forall pre expr lv,
+  hoare_lexpr pre expr lv ->
+  Hoare.hoare_lexpr ge this (to_shallow_assertion_continue pre) expr (lval_to_semlval lv).
 Proof.
   unfold Hoare.hoare_lexpr; intros.
   eapply eval_lexpr_sound; eassumption.
 Qed.
 
 Definition hoare_write (pre : assertion) (lv : Lval) (v : Val) (post : assertion) : Prop :=
-  is_writable_lval lv pre /\ eval_write pre lv v = post.
+  is_writable_lval lv (fst pre) /\ eval_write (fst pre) lv v = (fst post) /\ (snd pre = snd post).
 
-Lemma hoare_write_sound : forall p pre lv v post,
-  wellformed pre ->
-  hoare_write pre lv v post ->
-  Hoare.hoare_write p (to_shallow_assertion p pre) (lval_to_semlval lv) v (to_shallow_assertion p post).
+Lemma exec_write_preserve_extern_state : forall st lv v st',
+  exec_write (H := V1Model) this st lv v st' ->
+  snd st = snd st'.
 Proof.
-  unfold Hoare.hoare_write; intros. destruct H1; subst.
-  eapply eval_write_sound; try eassumption.
+  intros * H_exec_write.
+  induction H_exec_write; only 2-5 : assumption.
+  destruct st; destruct st'. inversion H. constructor.
 Qed.
+
+Lemma hoare_write_sound : forall pre lv v post,
+  wellformed (fst pre) ->
+  hoare_write pre lv v post ->
+  Hoare.hoare_write this (to_shallow_assertion_continue pre) (lval_to_semlval lv) v (to_shallow_assertion_continue post).
+Proof.
+  unfold Hoare.hoare_write; intros.
+  destruct pre; destruct post;
+    destruct st as [m es]; destruct st' as [m' es'];
+    destruct H0 as [? []]; destruct H1; simpl in *; subst.
+  split.
+  - eapply (eval_write_sound (H := V1Model)) with (st := (m, es)) (st' := (m', es')); eassumption.
+  - pose proof (exec_write_preserve_extern_state _ _ _ _ (ltac:(eassumption))).
+    scongruence.
+Qed.
+
+End WithThisPath.
 
 Inductive hoare_stmt : path -> assertion -> (@Statement tags_t) -> post_assertion -> Prop :=
   | hoare_stmt_assignment : forall p pre tags lhs rhs typ (post : post_assertion) lv v,
-      hoare_lexpr p pre lhs lv ->
-      is_valid_field pre lv ->
+      hoare_lexpr pre lhs lv ->
       hoare_expr pre rhs v ->
       hoare_write pre lv v post ->
       hoare_stmt p pre (MkStatement tags (StatAssignment lhs rhs) typ) post.
-
-Lemma hoare_stmt_sound : forall p pre stmt post,
-  wellformed pre ->
-  hoare_stmt p pre stmt post ->
-  Hoare.deep_hoare_stmt ge inst_m p (to_shallow_assertion p pre) stmt (to_shallow_post_assertion p post).
-Proof.
-  intros * H_wellformed H_hoare_stmt.
-  apply deep_hoare_stmt_intro.
-  induction H_hoare_stmt.
-  - hnf. intros. pinv @exec_stmt.
-    + repeat lazymatch goal with
-      | H : hoare_lexpr _ _ _ _ |- _ => apply hoare_lexpr_sound in H
-      | H : hoare_expr _ _ _ |- _ => apply hoare_expr_sound with (p := p) in H; only 2 : assumption
-      | H : hoare_write _ _ _ _ |- _ => eapply hoare_write_sound with (p := p) in H; only 2 : assumption
-      end.
-      specialize (H0 _ _ _ H4 H16) as [? H0]; subst sig0.
-      specialize (H2 _ _ H4 H15); subst v0.
-      eapply exec_write_congruent in H17. 3 : apply H0. 2 : { eapply state_is_valid_field_sound, is_valid_field_sound; eassumption. }
-      specialize (H3 _ _ H4 H17). simpl. destruct post; sfirstorder.
-    + pinv @exec_call; pinv hoare_expr.
-Qed.
 
 Inductive hoare_block : path -> assertion -> (@Block tags_t) -> post_assertion -> Prop :=
   | hoare_block_nil : forall p pre (post : post_assertion) tags,
@@ -111,20 +142,50 @@ Inductive hoare_block : path -> assertion -> (@Block tags_t) -> post_assertion -
       hoare_block p pre (BlockEmpty tags) post
   | hoare_block_cons : forall p pre stmt rest mid (post : post_assertion),
       hoare_stmt p pre stmt mid ->
-      wellformed mid ->
+      wellformed (fst (mid : assertion)) ->
       hoare_block p mid rest post ->
       hoare_block p pre (BlockCons stmt rest) post.
 
+Lemma hoare_stmt_sound : forall p pre stmt post,
+  wellformed (fst pre) ->
+  hoare_stmt p pre stmt post ->
+  Hoare.deep_hoare_stmt ge inst_m p (to_shallow_assertion_continue p pre) stmt (to_shallow_post_assertion p post).
+Proof.
+  intros * H_wellformed H_hoare_stmt.
+  apply deep_hoare_stmt_intro.
+  induction H_hoare_stmt.
+  - hnf. intros. pinv @exec_stmt.
+    + assert (is_valid_field (fst pre) lv). {
+        destruct H1. hauto unfold: is_true, is_writable_lval, andb, fst, assertion.
+      }
+      repeat lazymatch goal with
+      | H : hoare_lexpr _ _ _ |- _ => apply hoare_lexpr_sound with (this := p) in H
+      | H : hoare_expr _ _ _ |- _ => apply hoare_expr_sound with (this := p) in H; only 2 : assumption
+      | H : hoare_write _ _ _ _ |- _ => eapply hoare_write_sound with (this := p) in H; only 2 : assumption
+      end.
+      specialize (H _ _ _ H2 H14) as [? H]; subst sig0.
+      specialize (H0 _ _ H2 H13); subst v0.
+      eapply exec_write_congruent in H15.
+        3 : eassumption.
+        2 : {
+          destruct st; destruct pre; destruct H2.
+          eapply mem_is_valid_field_sound, is_valid_field_sound; eassumption.
+        }
+      specialize (H1 _ _ H2 H15). simpl. destruct post; sfirstorder.
+    + pinv @exec_call; pinv hoare_expr.
+    Unshelve. all : exact V1Model. (* try remove this *)
+Qed.
+
 Lemma hoare_block_sound : forall p pre block post,
-  wellformed pre ->
+  wellformed (fst pre) ->
   hoare_block p pre block post ->
-  Hoare.deep_hoare_block ge inst_m p (to_shallow_assertion p pre) block (to_shallow_post_assertion p post).
+  Hoare.deep_hoare_block ge inst_m p (to_shallow_assertion_continue p pre) block (to_shallow_post_assertion p post).
 Proof.
   intros * H_wellformed H_hoare_block.
   induction H_hoare_block.
   - constructor.
     destruct post. intros st ?; eapply implies_sound; eassumption.
-  - apply hoare_stmt_sound in H0; only 2 : assumption.
+  - apply hoare_stmt_sound in H; only 2 : assumption.
     destruct mid; econstructor; eauto.
 Qed.
 
